scaffolding correctness proofs for wp with leaps

deps/poulet4/lib/P4automata/Bisimulations/AlgorithmicLeapsProofs.v
@@ -2,12 +2,12 @@ Require Import Coq.Lists.List.
 Require Import Coq.Classes.EquivDec.
 Require Import Coq.Program.Equality.
 Import List.ListNotations.
-
 Require Import Poulet4.P4automata.P4automaton.
 Require Import Poulet4.FinType.
 Require Import Poulet4.P4automata.ConfRel.
 Require Import Poulet4.Relations.
-Require Poulet4.P4automata.WPSymLeap.
+Require Poulet4.P4automata.Bisimulations.Leaps.
+Require Import Poulet4.P4automata.Bisimulations.AlgorithmicLeaps.
 
 Section AlgorithmicLeaps.
   Variable (a: p4automaton).
@@ -21,22 +21,12 @@ Section AlgorithmicLeaps.
                           S q1 q2)
                         (at level 40).
 
-  Reserved Notation "R ⇝ S" (at level 10).
-  Inductive pre_bisimulation : rels conf -> rels conf -> rel conf :=
-  | PreBisimulationClose:
-      forall R q1 q2,
-        ⟦R⟧ q1 q2 ->
-        R ⇝ [] q1 q2
-  | PreBisimulationSkip:
-      forall R T (C: relation conf) q1 q2,
-        R ⊨ C ->
-        R ⇝ T q1 q2 ->
-        R ⇝ (C :: T) q1 q2
-  | PreBisimulationExtend:
-      forall R T C W q1 q2,
-        (C :: R) ⇝ (W ++ T) q1 q2 ->
-        (forall q1 q2, ⟦W⟧ q1 q2 -> (forall bit, C (step q1 bit) (step q2 bit))) ->
-        R ⇝ (C :: T) q1 q2
-  where "R ⇝ S" := (pre_bisimulation R S).
-
+  Lemma algorithmic_leaps_implies_bisimilar_leaps:
+    forall R T q1 q2,
+      pre_bisimulation a top R T q1 q2 ->
+      Leaps.bisimilar_with_leaps a q1 q2.
+  Proof.
+    intros.
+  Abort.
+  
 End AlgorithmicLeaps.
