deps/poulet4/lib/P4automata/Bisimulations/WPLeapsProofs.v
@@ -7,6 +7,7 @@ Require Import Poulet4.P4automata.P4automaton.
 Require Import Poulet4.FinType.
 Require Import Poulet4.P4automata.ConfRel.
 Require Import Poulet4.Relations.
+Require Import Poulet4.P4automata.Bisimulations.Leaps.
 Require Import Poulet4.P4automata.Bisimulations.WPLeaps.
 Require Import Poulet4.P4automata.Bisimulations.AlgorithmicProofs.
 
@@ -46,81 +47,16 @@ Section WPLeapsProofs.
   Notation "R ⊨ S" := (interp_entailment a top {| e_prem := R; e_concl := S |}) (at level 40).
   Notation δ := step.
 
-  Lemma ctopbbd_topbdd:
-    forall R,
-      ctopbdd a top R ->
-      topbdd a top ⟦R⟧.
+  Lemma wp_leaps_implies_bisim_leaps:
+    forall R T q1 q2,
+      pre_bisimulation a wp top R T q1 q2 ->
+      Leaps.bisimilar_with_leaps (P4A.interp a) q1 q2.
   Proof.
-    unfold ctopbdd, topbdd.
-    induction R; simpl; intros.
-    - assumption.
-    - inversion H1.
-      eauto.
-  Qed.
-
-  Lemma ctopbdd_app:
-    forall C T,
-      ctopbdd a top C ->
-      ctopbdd a top T ->
-      ctopbdd a top (C ++ T).
-  Proof.
-    unfold ctopbdd.
     intros.
-    rewrite in_app_iff in *.
-    intuition.
-  Qed.
-
-  Lemma topbdd_mono:
-    forall (R S: rel conf),
-      (forall x y, R x y -> S x y) ->
-      topbdd a top S ->
-      topbdd a top R.
-  Proof.
-    unfold topbdd.
-    auto.
-  Qed.
-
-  Lemma syn_pre_implies_sem_pre:
-    forall R S q1 q2,
-      pre_bisimulation a wp top R S q1 q2 ->
-      ctopbdd a top R ->
-      ctopbdd a top S ->
-      safe_wp_1bit a wp top ->
-      wp_bdd a wp top ->
-      Algorithmic.pre_bisimulation (P4A.interp a)
-                              top
-                              (map (interp_conf_rel a) R)
-                              (map (interp_conf_rel a) S)
-                              q1 q2.
-  Proof.
-    intros R S q1 q2 Hstep.
-    induction Hstep.
-    - simpl.
-      constructor.
-      eauto.
-    - simpl.
-      intros.
-      econstructor 2; eauto.
-      eapply IHHstep; eauto.
-      unfold ctopbdd; intros.
-      eauto with datatypes.
-    - rewrite map_app in IHHstep.
-      subst.
-      intros.
-      econstructor 3; eauto.
-      eapply IHHstep; eauto.
-      + unfold ctopbdd in *.
-        intros.
-        simpl (In _ _) in *.
-        intuition.
-      + eapply ctopbdd_app.
-        * eapply H5.
-          eapply H3.
-          eauto with datatypes.
-        * unfold ctopbdd in *; simpl (In _ _ ) in *; eauto.
-      + intros.
-        eapply H4; eauto.
-        eapply AlgorithmicProofs.interp_rels_top; eauto.
-  Qed.
+    cofix C.
+    constructor.
+    - admit.
+    - revert H0.
+  Abort.
 
 End WPLeapsProofs.
